xtext/org.archware.sosadl/src/org/archware/sosadl/validation/typing/impl/ArchitectureEnvContent.java
@@ -1,0 +1,16 @@
+package org.archware.sosadl.validation.typing.impl;
+
+import org.archware.sosadl.sosADL.ArchitectureDecl;
+import org.archware.sosadl.validation.typing.EnvContent;
+
+public class ArchitectureEnvContent implements EnvContent {
+	private final ArchitectureDecl architectureDecl;
+	
+	public ArchitectureEnvContent(ArchitectureDecl dtd) {
+		this.architectureDecl = dtd;
+	}
+	
+	public ArchitectureDecl getMediatorDecl() {
+		return this.architectureDecl;
+	}
+}
