xtext/org.archware.sosadl/src/org/archware/sosadl/validation/typing/impl/FunctionEnvContent.java
@@ -1,0 +1,18 @@
+package org.archware.sosadl.validation.typing.impl;
+
+import org.archware.sosadl.sosADL.FunctionDecl;
+import org.archware.sosadl.validation.typing.EnvContent;
+
+public class FunctionEnvContent implements EnvContent {
+	private final FunctionDecl function;
+
+	public FunctionEnvContent(FunctionDecl function) {
+		super();
+		this.function = function;
+	}
+
+	public FunctionDecl getFunction() {
+		return function;
+	}
+
+}
