xtext/org.archware.sosadl/src/org/archware/sosadl/validation/typing/impl/MediatorEnvContent.java
@@ -1,0 +1,16 @@
+package org.archware.sosadl.validation.typing.impl;
+
+import org.archware.sosadl.sosADL.MediatorDecl;
+import org.archware.sosadl.validation.typing.EnvContent;
+
+public class MediatorEnvContent implements EnvContent {
+	private final MediatorDecl mediatorDecl;
+	
+	public MediatorEnvContent(MediatorDecl dtd) {
+		this.mediatorDecl = dtd;
+	}
+	
+	public MediatorDecl getMediatorDecl() {
+		return this.mediatorDecl;
+	}
+}
