xtext/org.archware.sosadl/src/org/archware/sosadl/validation/typing/proof/Incrementally_nil.java
@@ -1,0 +1,17 @@
+package org.archware.sosadl.validation.typing.proof;
+
+import org.archware.sosadl.validation.typing.Environment;
+
+public class Incrementally_nil<T,P> implements Incrementally<T,P> {
+	@Mandatory private final Environment gamma;
+
+	public Incrementally_nil(Environment gamma) {
+		super();
+		this.gamma = gamma;
+	}
+
+	public Environment getGamma() {
+		return gamma;
+	}
+
+}
