xtext/org.archware.sosadl/src/org/archware/sosadl/validation/typing/proof/Mutually_all.java
@@ -1,0 +1,54 @@
+package org.archware.sosadl.validation.typing.proof;
+
+import java.util.List;
+
+import org.archware.sosadl.validation.typing.Environment;
+
+public class Mutually_all<T,P> implements Mutually<T,P> {
+	@Mandatory private final Environment gamma;
+	
+	private final List<T> l;
+	
+	@Mandatory private final Environment gamma1;
+	
+	@Mandatory private final Equality p1;
+	
+	@Mandatory private final Equality p2;
+	
+	@Mandatory private final Forall<T, P> p3;
+
+	public Mutually_all(Environment gamma, List<T> l, Environment gamma1, Equality p1, Equality p2, Forall<T, P> p3) {
+		super();
+		this.gamma = gamma;
+		this.l = l;
+		this.gamma1 = gamma1;
+		this.p1 = p1;
+		this.p2 = p2;
+		this.p3 = p3;
+	}
+
+	public Environment getGamma() {
+		return gamma;
+	}
+
+	public List<T> getL() {
+		return l;
+	}
+
+	public Environment getGamma1() {
+		return gamma1;
+	}
+
+	public Equality getP1() {
+		return p1;
+	}
+
+	public Equality getP2() {
+		return p2;
+	}
+
+	public Forall<T, P> getP3() {
+		return p3;
+	}
+
+}
