xtext/org.archware.sosadl/src/org/archware/sosadl/validation/typing/proof/Type_SystemDecl_datatype_Some.java
@@ -4,41 +4,44 @@ import org.archware.sosadl.sosADL.AssertionDecl;
 import org.archware.sosadl.sosADL.BehaviorDecl;
 import org.archware.sosadl.sosADL.DataType;
 import org.archware.sosadl.sosADL.DataTypeDecl;
-import org.archware.sosadl.sosADL.FormalParameter;
+import org.archware.sosadl.sosADL.FunctionDecl;
 import org.archware.sosadl.sosADL.GateDecl;
 import org.archware.sosadl.validation.typing.Environment;
 import org.eclipse.emf.common.util.EList;
 
-public class Type_SystemDecl implements Type_system {
+public class Type_SystemDecl_datatype_Some implements Type_systemblock {
 	@Mandatory private final Environment gamma;
 	
 	@Mandatory private final String name;
 	
-	private final EList<FormalParameter> params;
+	@Mandatory private final String d_name;
 	
-	@Mandatory private final Environment gamma1;
+	@Mandatory private final DataType d_def;
 	
-	private final EList<DataTypeDecl> datatypes;
+	private final EList<FunctionDecl> d_funs;
+	
+	private final EList<DataTypeDecl> l;
 	
 	private final EList<GateDecl> gates;
-
+	
 	@Mandatory private final BehaviorDecl bhv;
 	
 	private final AssertionDecl assrt;
 	
-	@Mandatory private final Mutually<FormalParameter, Ex<DataType, And<Equality,Type_datatype>>> p1;
+	@Mandatory private final Type_datatypeDecl p1;
 	
 	@Mandatory private final Type_systemblock p2;
 
-	public Type_SystemDecl(Environment gamma, String name, EList<FormalParameter> params, Environment gamma1,
-			EList<DataTypeDecl> datatypes, EList<GateDecl> gates, BehaviorDecl bhv, AssertionDecl assrt,
-			Mutually<FormalParameter, Ex<DataType, And<Equality, Type_datatype>>> p1, Type_systemblock p2) {
+	public Type_SystemDecl_datatype_Some(Environment gamma, String name, String d_name, DataType d_def,
+			EList<FunctionDecl> d_funs, EList<DataTypeDecl> l, EList<GateDecl> gates, BehaviorDecl bhv,
+			AssertionDecl assrt, Type_datatypeDecl p1, Type_systemblock p2) {
 		super();
 		this.gamma = gamma;
 		this.name = name;
-		this.params = params;
-		this.gamma1 = gamma1;
-		this.datatypes = datatypes;
+		this.d_name = d_name;
+		this.d_def = d_def;
+		this.d_funs = d_funs;
+		this.l = l;
 		this.gates = gates;
 		this.bhv = bhv;
 		this.assrt = assrt;
@@ -54,16 +57,20 @@ public class Type_SystemDecl implements Type_system {
 		return name;
 	}
 
-	public EList<FormalParameter> getParams() {
-		return params;
+	public String getD_name() {
+		return d_name;
 	}
 
-	public Environment getGamma1() {
-		return gamma1;
+	public DataType getD_def() {
+		return d_def;
 	}
 
-	public EList<DataTypeDecl> getDatatypes() {
-		return datatypes;
+	public EList<FunctionDecl> getD_funs() {
+		return d_funs;
+	}
+
+	public EList<DataTypeDecl> getL() {
+		return l;
 	}
 
 	public EList<GateDecl> getGates() {
@@ -78,7 +85,7 @@ public class Type_SystemDecl implements Type_system {
 		return assrt;
 	}
 
-	public Mutually<FormalParameter, Ex<DataType, And<Equality, Type_datatype>>> getP1() {
+	public Type_datatypeDecl getP1() {
 		return p1;
 	}
 
